Changed computation of ghosts until pass 2 of resolution. Other clean-up in resolution passes, like: Include everything of type "char" into bounds that are discovered, and likewise for reference types. Allow more set comprehensions, determining if they are finite based on their argument type. Changed CalcExpr.SubExpressions to not include computed expressions.

Binaries/DafnyRuntime.cs
@@ -1012,6 +1012,12 @@ namespace Dafny
         return pred(false) || pred(true);
       }
     }
+    public static bool QuantChar(bool frall, System.Predicate<char> pred) {
+      for (int i = 0; i < 0x10000; i++) {
+        if (pred((char)i) != frall) { return !frall; }
+      }
+      return frall;
+    }
     public static bool QuantInt(BigInteger lo, BigInteger hi, bool frall, System.Predicate<BigInteger> pred) {
       for (BigInteger i = lo; i < hi; i++) {
         if (pred(i) != frall) { return !frall; }
@@ -1049,6 +1055,13 @@ namespace Dafny
       get {
         yield return false;
         yield return true;
+      }
+    }
+    public static IEnumerable<char> AllChars {
+      get {
+        for (int i = 0; i < 0x10000; i++) {
+          yield return (char)i;
+        }
       }
     }
     public static IEnumerable<BigInteger> AllIntegers {
