Source/Dafny/Cloner.cs
@@ -550,13 +550,21 @@ namespace Microsoft.Dafny
         r = new ForallStmt(Tok(s.Tok), Tok(s.EndTok), s.BoundVars.ConvertAll(CloneBoundVar), null, CloneExpr(s.Range), s.Ens.ConvertAll(CloneMayBeFreeExpr), CloneStmt(s.Body));
 
       } else if (stmt is CalcStmt) {
-          var s = (CalcStmt)stmt;
-          r = new CalcStmt(Tok(s.Tok), Tok(s.EndTok), CloneCalcOp(s.Op), s.Lines.ConvertAll(CloneExpr), s.Hints.ConvertAll(CloneBlockStmt), s.StepOps.ConvertAll(CloneCalcOp), CloneCalcOp(s.ResultOp), CloneAttributes(s.Attributes));
+        var s = (CalcStmt)stmt;
+        // calc statements have the unusual property that the last line is duplicated.  If that is the case (which
+        // we expect it to be here), we share the clone of that line as well.
+        var lineCount = s.Lines.Count;
+        var lines = new List<Expression>(lineCount);
+        for (int i = 0; i < lineCount; i++) {
+          lines.Add(i == lineCount - 1 && 2 <= lineCount && s.Lines[i] == s.Lines[i - 1] ? lines[i - 1] : CloneExpr(s.Lines[i]));
+        }
+        Contract.Assert(lines.Count == lineCount);
+        r = new CalcStmt(Tok(s.Tok), Tok(s.EndTok), CloneCalcOp(s.Op), lines, s.Hints.ConvertAll(CloneBlockStmt), s.StepOps.ConvertAll(CloneCalcOp), CloneCalcOp(s.ResultOp), CloneAttributes(s.Attributes));
 
       } else if (stmt is MatchStmt) {
         var s = (MatchStmt)stmt;
         r = new MatchStmt(Tok(s.Tok), Tok(s.EndTok), CloneExpr(s.Source),
-          s.Cases.ConvertAll(CloneMatchCaseStmt), s.UsesOptionalBraces);
+        s.Cases.ConvertAll(CloneMatchCaseStmt), s.UsesOptionalBraces);
 
       } else if (stmt is AssignSuchThatStmt) {
         var s = (AssignSuchThatStmt)stmt;
